Experiments

Weidenbach_Book/IsaSAT/IsaSAT_EVSIDS.thy
@@ -5,92 +5,96 @@ theory IsaSAT_EVSIDS
     IsaSAT_EVSIDS_double
 begin
 
-section \<open>VSIDS\<close>
-(*TODO: Missing invariant? \<open>Max ({0} \<union> w ` set_mset b) \<le> vsids_limit\<close> *)
-(*We can try to re-use m as the increment inc*)
-type_synonym ('a, 'v) vsids = \<open>('a multiset \<times> 'a multiset \<times> ('a \<Rightarrow> 'v)) \<times> 'v\<close>
-definition vsids :: \<open>'a multiset \<Rightarrow> ('a, 'ann) ann_lits \<Rightarrow> ('a, 'v::{zero,linorder}) vsids set\<close> where
-\<open>vsids \<A> M = {((\<B>, b, w), inc). set_mset \<B> = set_mset \<A> \<and> b \<subseteq># \<A> \<and> (\<forall>L \<in>#\<A>. L \<notin># b \<longrightarrow> defined_lit M (Pos L)) \<and> distinct_mset b}\<close>
+section \<open>EVSIDS\<close>
 
-lemma vsids_prepend: \<open>vc \<in> vsids \<A> M \<Longrightarrow> vc \<in> vsids \<A> (L # M)\<close>
-  unfolding vsids_def by (auto simp: defined_lit_map)
+type_synonym ('a, 'v) evsids = \<open>('a multiset \<times> 'a multiset \<times> ('a \<Rightarrow> 'v)) \<times> 'v\<close>
+definition evsids :: \<open>'a multiset \<Rightarrow> ('a, 'ann) ann_lits \<Rightarrow> ('a, double\<^sub>p) evsids set\<close> where
+\<open>evsids \<A> M = {((\<B>, b, w), inc). set_mset \<B> = set_mset \<A> \<and> b \<subseteq># \<A> \<and> (inc \<le> evsids_limit) \<and> (\<forall>L\<in>#\<A>. w L \<le> evsids_limit) \<and> (\<forall>L \<in>#\<A>. L \<notin># b \<longrightarrow> defined_lit M (Pos L)) \<and> distinct_mset b}\<close>
 
-interpretation VSIDS: hmstruct_with_prio where
+lemma evsids_prepend: \<open>vc \<in> evsids \<A> M \<Longrightarrow> vc \<in> evsids \<A> (L # M)\<close>
+  unfolding evsids_def by (auto simp: defined_lit_map)
+
+interpretation EVSIDS: hmstruct_with_prio where
   le = \<open>(\<ge>) :: double\<^sub>p \<Rightarrow> double\<^sub>p \<Rightarrow> bool\<close> and
   lt = \<open>(>)\<close>
   apply unfold_locales
-  subgoal using double\<^sub>p_le_iff_le_or_eq by auto
-  subgoal using transp_def double\<^sub>p_trans_le by auto
-  subgoal using transp_def double\<^sub>p_trans_lt by auto
-  subgoal using double\<^sub>p_total_lt by (simp add: totalpI)
+  subgoal by auto
+  subgoal by auto
+  subgoal by auto
+  subgoal by auto
   done
 
-definition vsids_tl_pre :: \<open>'a \<Rightarrow> ('a, 'v) vsids \<Rightarrow> bool\<close> where
-  \<open>vsids_tl_pre L = (\<lambda>(vc, inc). L \<in># fst vc)\<close>
+definition evsids_tl_pre :: \<open>'a \<Rightarrow> ('a, 'v) evsids \<Rightarrow> bool\<close> where
+  \<open>evsids_tl_pre L = (\<lambda>(vc, m). L \<in># fst vc)\<close>
 
-definition vsids_tl :: \<open>'a \<Rightarrow> ('a, 'v::ord) vsids \<Rightarrow> ('a, 'v) vsids nres\<close> where
-  \<open>vsids_tl L = (\<lambda>(vc, inc). do {
-    ASSERT (vsids_tl_pre L (vc, inc));
-    vc \<leftarrow> VSIDS.mop_prio_insert_unchanged L vc;
-    RETURN (vc, inc)
+definition evsids_tl :: \<open>'a \<Rightarrow> ('a, double\<^sub>p) evsids \<Rightarrow> ('a, double\<^sub>p) evsids nres\<close> where
+  \<open>evsids_tl L = (\<lambda>(vc, inc). do {
+    ASSERT (evsids_tl_pre L (vc, inc));
+    b \<leftarrow> EVSIDS.mop_prio_is_in L vc;
+    if \<not>b then do {
+      w \<leftarrow> EVSIDS.mop_prio_old_weight L vc;
+      let w = (if w \<le> evsids_limit then w else evsids_limit);
+      vc \<leftarrow> EVSIDS.mop_prio_insert L w vc;
+      RETURN (vc, inc)
+    } else RETURN (vc, inc)
   })\<close>
 
-lemma vsids_tl:
-  \<open>vc \<in> vsids \<A> M \<Longrightarrow> L \<in># \<A> \<Longrightarrow> M \<noteq> [] \<Longrightarrow> L = atm_of (lit_of (hd M)) \<Longrightarrow> vsids_tl L vc \<le> RES (vsids \<A> (tl M))\<close>
-  unfolding vsids_tl_def VSIDS.mop_prio_insert_unchanged_def
-    VSIDS.mop_prio_insert_raw_unchanged_def nres_monad3
-    VSIDS.mop_prio_is_in_def
-    VSIDS.mop_prio_old_weight_def
-    VSIDS.mop_prio_insert_def RES_RES_RETURN_RES RETURN_def
-    VSIDS.mop_prio_old_weight_def case_prod_beta nres_monad1
+lemma evsids_tl:
+  \<open>vc \<in> evsids \<A> M \<Longrightarrow> L \<in># \<A> \<Longrightarrow> M \<noteq> [] \<Longrightarrow> L = atm_of (lit_of (hd M)) \<Longrightarrow> evsids_tl L vc \<le> RES (evsids \<A> (tl M))\<close>
+  unfolding evsids_tl_def EVSIDS.mop_prio_insert_unchanged_def
+    EVSIDS.mop_prio_insert_raw_unchanged_def nres_monad3
+    EVSIDS.mop_prio_is_in_def
+    EVSIDS.mop_prio_old_weight_def
+    EVSIDS.mop_prio_insert_def RES_RES_RETURN_RES RETURN_def
+    EVSIDS.mop_prio_old_weight_def case_prod_beta nres_monad1
   apply (refine_vcg lhs_step_If)
   subgoal
-    by (cases M) (auto simp: vsids_def VSIDS.mop_prio_insert_unchanged_def insert_subset_eq_iff
-        vsids_tl_pre_def
+    by (cases M) (auto simp: evsids_def EVSIDS.mop_prio_insert_unchanged_def insert_subset_eq_iff
+        evsids_tl_pre_def
       intro!: subset_add_mset_notin_subset)
   subgoal
-    by (auto simp: vsids_def VSIDS.mop_prio_insert_unchanged_def insert_subset_eq_iff
-        vsids_tl_pre_def
+    by (auto simp: evsids_def EVSIDS.mop_prio_insert_unchanged_def insert_subset_eq_iff
+        evsids_tl_pre_def
       intro!: subset_add_mset_notin_subset)
   subgoal
-    apply (auto simp: vsids_def VSIDS.mop_prio_insert_unchanged_def RES_RES_RETURN_RES
-      defined_lit_map vsids_tl_pre_def dest: subset_add_mset_notin_subset
+    apply (auto simp: evsids_def EVSIDS.mop_prio_insert_unchanged_def RES_RES_RETURN_RES
+      defined_lit_map evsids_tl_pre_def dest: subset_add_mset_notin_subset
       dest: multi_member_split)
     apply (smt (verit, best) image_iff not_hd_in_tl)
-     apply (metis mset_subset_eq_add_mset_cancel multi_member_split subset_add_mset_notin_subset)
-    by (smt (verit, ccfv_threshold) imageE imageI not_hd_in_tl)
+      apply (metis mset_add mset_subset_eq_add_mset_cancel subset_add_mset_notin_subset)
+    by (smt (verit, ccfv_threshold) image_iff in_hd_or_tl_conv)
   done
 
-definition vsids_get_min :: \<open>('a, double\<^sub>p) vsids \<Rightarrow> 'a nres\<close> where
-  \<open>vsids_get_min = (\<lambda>(vc, inc). do {
-    L \<leftarrow> VSIDS.mop_prio_peek_min vc;
+definition evsids_get_min :: \<open>('a, double\<^sub>p) evsids \<Rightarrow> 'a nres\<close> where
+  \<open>evsids_get_min = (\<lambda>(vc, m). do {
+    L \<leftarrow> EVSIDS.mop_prio_peek_min vc;
     RETURN L
   })\<close>
 
-definition vsids_mset :: \<open>('a, 'v) vsids \<Rightarrow> _\<close> where
-  \<open>vsids_mset x = fst (snd (fst x))\<close>
+definition evsids_mset :: \<open>('a, 'v) evsids \<Rightarrow> _\<close> where
+  \<open>evsids_mset x = fst (snd (fst x))\<close>
 
-lemma vsids_get_min:
-  \<open>vsids_mset x \<noteq> {#} \<Longrightarrow> vsids_get_min x \<le> SPEC (\<lambda>v. VSIDS.prio_peek_min (fst x) v)\<close>
-  unfolding vsids_get_min_def VSIDS.mop_prio_peek_min_def vsids_mset_def
-  by refine_vcg (auto simp: VSIDS.prio_peek_min_def)
+lemma evsids_get_min:
+  \<open>evsids_mset x \<noteq> {#} \<Longrightarrow> evsids_get_min x \<le> SPEC (\<lambda>v. EVSIDS.prio_peek_min (fst x) v)\<close>
+  unfolding evsids_get_min_def EVSIDS.mop_prio_peek_min_def evsids_mset_def
+  by refine_vcg (auto simp: EVSIDS.prio_peek_min_def)
 
-definition vsids_pop_min :: \<open>('a, double\<^sub>p) vsids \<Rightarrow> ('a \<times> ('a, double\<^sub>p) vsids) nres\<close> where
-  \<open>vsids_pop_min = (\<lambda>(vc, inc). do {
-    (v, vc) \<leftarrow> VSIDS.mop_prio_pop_min vc;
+definition evsids_pop_min :: \<open>('a, double\<^sub>p) evsids \<Rightarrow> ('a \<times> ('a, double\<^sub>p) evsids) nres\<close> where
+  \<open>evsids_pop_min = (\<lambda>(vc, inc). do {
+    (v, vc) \<leftarrow> EVSIDS.mop_prio_pop_min vc;
     RETURN (v, (vc, inc))
   })\<close>
 
-definition vsids_find_next_undef :: \<open>nat multiset \<Rightarrow> (nat, double\<^sub>p) vsids \<Rightarrow> (nat, nat) ann_lits \<Rightarrow> (nat option \<times> (nat, double\<^sub>p) vsids) nres\<close> where
-\<open>vsids_find_next_undef \<A> = (\<lambda>vc M. do {
+definition evsids_find_next_undef :: \<open>nat multiset \<Rightarrow> (nat, double\<^sub>p) evsids \<Rightarrow> (nat, nat) ann_lits \<Rightarrow> (nat option \<times> (nat, double\<^sub>p) evsids) nres\<close> where
+\<open>evsids_find_next_undef \<A> = (\<lambda>vc M. do {
   WHILE\<^sub>T\<^bsup>(\<lambda>(L, vc).
-        (L = None \<longrightarrow> vc \<in> vsids \<A> M) \<and>
-        (L \<noteq> None \<longrightarrow> vc \<in> vsids \<A> (Decided (Pos (the L)) # M) \<and> Pos (the L) \<in># \<L>\<^sub>a\<^sub>l\<^sub>l \<A> \<and> undefined_lit M (Pos (the L))))
+        (L = None \<longrightarrow> vc \<in> evsids \<A> M) \<and>
+        (L \<noteq> None \<longrightarrow> vc \<in> evsids \<A> (Decided (Pos (the L)) # M) \<and> Pos (the L) \<in># \<L>\<^sub>a\<^sub>l\<^sub>l \<A> \<and> undefined_lit M (Pos (the L))))
   \<^esup>
-      (\<lambda>(nxt, vc). nxt = None \<and> vsids_mset vc \<noteq> {#})
+      (\<lambda>(nxt, vc). nxt = None \<and> evsids_mset vc \<noteq> {#})
       (\<lambda>(a, vc). do {
          ASSERT (a = None);
-         (L, vc) \<leftarrow> vsids_pop_min vc;
+         (L, vc) \<leftarrow> evsids_pop_min vc;
          ASSERT(Pos L \<in># \<L>\<^sub>a\<^sub>l\<^sub>l  \<A>);
          if defined_lit M (Pos L) then RETURN (None, vc)
          else RETURN (Some L, vc)
@@ -99,53 +103,53 @@ definition vsids_find_next_undef :: \<open>nat multiset \<Rightarrow> (nat, doub
       (None, vc)
   })\<close>
 
-lemma vsids_pop_min:
-  \<open>vsids_mset x \<noteq> {#} \<Longrightarrow> x \<in> vsids \<A> M \<Longrightarrow>
-  vsids_pop_min x \<le> SPEC (\<lambda>(v, vc). vsids_mset vc = vsids_mset x - {#v#} \<and> v \<in># vsids_mset x \<and>
-    VSIDS.prio_peek_min (fst x) v \<and>
-    (defined_lit M (Pos v) \<longrightarrow> vc \<in> vsids \<A> M) \<and>
-    (undefined_lit M (Pos v) \<longrightarrow> vc \<in> vsids \<A> (Decided (Pos v) # M)))\<close>
-  unfolding VSIDS.mop_prio_pop_min_def vsids_pop_min_def
-    VSIDS.mop_prio_peek_min_def VSIDS.mop_prio_del_def
+lemma evsids_pop_min:
+  \<open>evsids_mset x \<noteq> {#} \<Longrightarrow> x \<in> evsids \<A> M \<Longrightarrow>
+  evsids_pop_min x \<le> SPEC (\<lambda>(v, vc). evsids_mset vc = evsids_mset x - {#v#} \<and> v \<in># evsids_mset x \<and>
+    EVSIDS.prio_peek_min (fst x) v \<and>
+    (defined_lit M (Pos v) \<longrightarrow> vc \<in> evsids \<A> M) \<and>
+    (undefined_lit M (Pos v) \<longrightarrow> vc \<in> evsids \<A> (Decided (Pos v) # M)))\<close>
+  unfolding EVSIDS.mop_prio_pop_min_def evsids_pop_min_def
+    EVSIDS.mop_prio_peek_min_def EVSIDS.mop_prio_del_def
   by refine_vcg
-   (auto simp: vsids_def VSIDS.prio_peek_min_def distinct_mset_remove1_All VSIDS.prio_del_def
-      defined_lit_map vsids_mset_def dest: in_diffD)
+   (auto simp: evsids_def EVSIDS.prio_peek_min_def distinct_mset_remove1_All EVSIDS.prio_del_def
+      defined_lit_map evsids_mset_def dest: in_diffD)
 
-lemma vsids_find_next_undef:
+lemma evsids_find_next_undef:
   assumes
-    vmtf: \<open>vc \<in> vsids \<A> M\<close>
-  shows \<open>vsids_find_next_undef \<A> vc M
+    vmtf: \<open>vc \<in> evsids \<A> M\<close>
+  shows \<open>evsids_find_next_undef \<A> vc M
      \<le> \<Down> Id (SPEC (\<lambda>(L, vc).
-        (L = None \<longrightarrow> vc \<in> vsids \<A> M \<and> (\<forall>L\<in>#\<L>\<^sub>a\<^sub>l\<^sub>l \<A>. defined_lit M L)) \<and>
-        (L \<noteq> None \<longrightarrow> vc \<in> vsids \<A> (Decided (Pos (the L)) # M) \<and> Pos (the L) \<in># \<L>\<^sub>a\<^sub>l\<^sub>l \<A> \<and> undefined_lit M (Pos (the L)))))\<close>
+        (L = None \<longrightarrow> vc \<in> evsids \<A> M \<and> (\<forall>L\<in>#\<L>\<^sub>a\<^sub>l\<^sub>l \<A>. defined_lit M L)) \<and>
+        (L \<noteq> None \<longrightarrow> vc \<in> evsids \<A> (Decided (Pos (the L)) # M) \<and> Pos (the L) \<in># \<L>\<^sub>a\<^sub>l\<^sub>l \<A> \<and> undefined_lit M (Pos (the L)))))\<close>
 proof -
-  have [refine0]: \<open>wf (measure (\<lambda>(_, vc). size (vsids_mset vc)))\<close>
+  have [refine0]: \<open>wf (measure (\<lambda>(_, vc). size (evsids_mset vc)))\<close>
     by auto
   show ?thesis
-    unfolding vsids_find_next_undef_def
-    apply (refine_vcg vsids_pop_min[of _ \<A> M, THEN order_trans])
+    unfolding evsids_find_next_undef_def
+    apply (refine_vcg evsids_pop_min[of _ \<A> M, THEN order_trans])
     subgoal using assms by auto
     subgoal by auto
-    subgoal by (auto simp: VSIDS.prio_peek_min_def vsids_def vsids_mset_def
+    subgoal by (auto simp: EVSIDS.prio_peek_min_def evsids_def evsids_mset_def
       in_\<L>\<^sub>a\<^sub>l\<^sub>l_atm_of_\<A>\<^sub>i\<^sub>n)
     subgoal by auto
     subgoal by auto
     subgoal by auto
     subgoal by auto
-    subgoal by (auto simp: vsids_def VSIDS.prio_peek_min_def
+    subgoal by (auto simp: evsids_def EVSIDS.prio_peek_min_def
       in_\<L>\<^sub>a\<^sub>l\<^sub>l_atm_of_\<A>\<^sub>i\<^sub>n)
     subgoal by auto
     subgoal by auto
     subgoal by auto
     subgoal by auto
-    subgoal by (auto simp: VSIDS.prio_peek_min_def vsids_mset_def dest: multi_member_split)
+    subgoal by (auto simp: EVSIDS.prio_peek_min_def evsids_mset_def dest: multi_member_split)
     subgoal by auto
     subgoal by auto
     subgoal by auto
     subgoal by auto
-    subgoal by (auto simp: VSIDS.prio_peek_min_def vsids_mset_def dest: multi_member_split)
+    subgoal by (auto simp: EVSIDS.prio_peek_min_def evsids_mset_def dest: multi_member_split)
     subgoal by auto
-    subgoal by (auto simp: VSIDS.prio_peek_min_def vsids_mset_def vsids_def
+    subgoal by (auto simp: EVSIDS.prio_peek_min_def evsids_mset_def evsids_def
       in_\<L>\<^sub>a\<^sub>l\<^sub>l_atm_of_\<A>\<^sub>i\<^sub>n dest!: multi_member_split[of \<open>_ :: nat\<close>])
     subgoal by auto
     subgoal by auto
@@ -153,86 +157,112 @@ proof -
     done
 qed
 
-definition vsids_push_literal_pre where
-  \<open>vsids_push_literal_pre \<A> L = (\<lambda>vc. L \<in># \<A>)\<close>
+(*TODO: Rescaling*)
+definition evsids_rescale :: \<open>('a, double\<^sub>p) evsids \<Rightarrow> ('a, double\<^sub>p) evsids\<close> where
+  \<open>evsids_rescale = (\<lambda>((\<B>, b, w), inc).
+     ((\<B>, b, \<lambda>L. let x = w L * evsids_rescale_factor in if x \<le> evsids_limit then x else evsids_limit),
+      (let i = inc * evsids_rescale_factor in if i \<le> evsids_limit then i else evsids_limit)))\<close>
 
-definition vsids_push_literal :: \<open>'a \<Rightarrow> ('a, double\<^sub>p) vsids \<Rightarrow> ('a, double\<^sub>p) vsids nres\<close> where
-  \<open>vsids_push_literal L = (\<lambda>(vc, inc). do {
-  ASSERT (L \<in># fst vc);
-  w \<leftarrow> VSIDS.mop_prio_old_weight L vc;
-  let w = w + inc;
-  vc \<leftarrow> VSIDS.mop_prio_insert_maybe L w vc;
-  RETURN (vc, inc)
+lemma evsids_rescale_in_evsids:
+  assumes "set_mset \<B> = set_mset \<A>" and "b \<subseteq># \<A>"
+    and "\<forall>L \<in>#\<A>. L \<notin># b \<longrightarrow> defined_lit M (Pos L)" and "distinct_mset b"
+  shows \<open>evsids_rescale ((\<B>, b, w), inc) \<in> evsids \<A> M\<close>
+  using assms unfolding evsids_rescale_def evsids_def apply (auto simp: Let_def) done
+
+definition evsids_push_literal_pre where
+  \<open>evsids_push_literal_pre \<A> L = (\<lambda>vc. L \<in># \<A>)\<close>
+
+definition evsids_push_literal :: \<open>nat \<Rightarrow> (nat, double\<^sub>p) evsids \<Rightarrow> (nat, double\<^sub>p) evsids nres\<close> where
+  \<open>evsids_push_literal L = (\<lambda>(vc, inc). do {
+    ASSERT (L \<in># fst vc);
+    w \<leftarrow> EVSIDS.mop_prio_old_weight L vc;
+    let w = (if w \<le> evsids_limit then w else evsids_limit);
+    let w' = w + inc;
+    vc \<leftarrow> EVSIDS.mop_prio_insert_maybe L w' vc;
+    if evsids_limit < w' then RETURN (evsids_rescale (vc, inc))
+    else RETURN (vc, inc)
   })\<close>
 
-lemma vsids_push_literal:
-  \<open>vc \<in> vsids \<A> M \<Longrightarrow> vsids_push_literal_pre \<A> L vc \<Longrightarrow> vsids_push_literal L vc \<le> SPEC (\<lambda>vc. vc \<in> vsids \<A> M)\<close>
-  unfolding vsids_push_literal_def VSIDS.mop_prio_insert_maybe_def
-    VSIDS.mop_prio_old_weight_def vsids_push_literal_pre_def
-    VSIDS.mop_prio_insert_def VSIDS.mop_prio_change_weight_def
-    VSIDS.mop_prio_is_in_def
+lemma evsids_push_literal:
+  \<open>vc \<in> evsids \<A> M \<Longrightarrow> evsids_push_literal_pre \<A> L vc \<Longrightarrow> evsids_push_literal L vc \<le> SPEC (\<lambda>vc. vc \<in> evsids \<A> M)\<close>
+  unfolding evsids_push_literal_def EVSIDS.mop_prio_insert_maybe_def
+    EVSIDS.mop_prio_old_weight_def evsids_push_literal_pre_def
+    EVSIDS.mop_prio_insert_def EVSIDS.mop_prio_change_weight_def
+    EVSIDS.mop_prio_is_in_def
   apply refine_vcg
-  subgoal by (auto simp: vsids_def vsids_mset_def)
-  subgoal by (auto simp: vsids_def dest!: multi_member_split)
-  subgoal by (auto simp: VSIDS.mop_prio_change_weight_def vsids_def
+  subgoal by (auto simp: evsids_def evsids_mset_def)
+  subgoal by (auto simp: evsids_def dest!: multi_member_split)
+  subgoal by (auto simp: EVSIDS.mop_prio_change_weight_def evsids_def
     dest!: multi_member_split)
-  subgoal by (auto simp: vsids_def dest!: multi_member_split)
-  subgoal by (auto simp: vsids_def vsids_mset_def)
-  subgoal by (auto simp: vsids_def vsids_mset_def dest!: multi_member_split
+  subgoal by (auto simp: evsids_def dest!: multi_member_split)
+  subgoal by (auto simp: evsids_def evsids_mset_def)
+  subgoal by (auto simp: evsids_def evsids_mset_def dest!: multi_member_split
     dest: subset_add_mset_notin_subset)
-  subgoal by (auto simp: vsids_def vsids_mset_def dest!: multi_member_split
+  subgoal by (auto simp: evsids_def evsids_mset_def dest!: multi_member_split
     dest: subset_add_mset_notin_subset)
-  subgoal by (auto simp: vsids_def vsids_mset_def dest!: multi_member_split
+  subgoal by (auto simp: evsids_def evsids_mset_def dest!: multi_member_split
     dest: subset_add_mset_notin_subset)
-  subgoal using double_plus\<^sub>p_mono by auto 
-  subgoal by (auto simp: vsids_def vsids_mset_def dest!: multi_member_split
+  subgoal by (auto simp: evsids_def evsids_mset_def dest!: multi_member_split
     dest: subset_add_mset_notin_subset)
-  subgoal by (auto simp: vsids_def vsids_mset_def dest!: multi_member_split
+  subgoal using double_plus\<^sub>p_mono by (auto split: if_splits; simp add: evsids_def)
+  subgoal
+  by (rule evsids_rescale_in_evsids;
+      auto simp: evsids_def evsids_mset_def dest!: multi_member_split
+        dest: subset_add_mset_notin_subset) 
+  subgoal by (auto simp: evsids_def evsids_mset_def dest!: multi_member_split
     dest: subset_add_mset_notin_subset)
-  subgoal by (auto simp: vsids_def vsids_mset_def dest!: multi_member_split
+  subgoal by (auto simp: evsids_def evsids_mset_def dest!: multi_member_split
     dest: subset_add_mset_notin_subset)
-  subgoal by (auto simp: vsids_def vsids_mset_def dest!: multi_member_split
+  subgoal by (auto simp: evsids_def evsids_mset_def dest!: multi_member_split
     dest: subset_add_mset_notin_subset)
-  subgoal by (auto simp: vsids_def vsids_mset_def dest!: multi_member_split
+  subgoal by (auto simp: evsids_def evsids_mset_def dest!: multi_member_split
     dest: subset_add_mset_notin_subset)
-  subgoal by (auto simp: vsids_def vsids_mset_def dest!: multi_member_split
+  subgoal
+          by (rule evsids_rescale_in_evsids;
+            auto simp: evsids_def evsids_mset_def dest!: multi_member_split
+              dest: subset_add_mset_notin_subset)
+  subgoal by (auto simp: evsids_def evsids_mset_def dest!: multi_member_split
     dest: subset_add_mset_notin_subset)
-  subgoal by (auto simp: vsids_def vsids_mset_def dest!: multi_member_split
+  subgoal by (auto simp: evsids_def evsids_mset_def dest!: multi_member_split
     dest: subset_add_mset_notin_subset)
-  subgoal by (auto simp: vsids_def vsids_mset_def dest!: multi_member_split
+  subgoal by (auto simp: evsids_def evsids_mset_def dest!: multi_member_split
+    dest: subset_add_mset_notin_subset)
+  subgoal by (auto simp: evsids_def evsids_mset_def dest!: multi_member_split
+    dest: subset_add_mset_notin_subset)
+  subgoal by (auto simp: evsids_def evsids_mset_def dest!: multi_member_split
     dest: subset_add_mset_notin_subset)
   done
 
-definition vsids_flush_int :: \<open>nat multiset \<Rightarrow> (nat,nat) ann_lits \<Rightarrow> (nat, double\<^sub>p) vsids \<Rightarrow> _ \<Rightarrow> ((nat, double\<^sub>p) vsids \<times> _)nres\<close> where
-\<open>vsids_flush_int \<A>\<^sub>i\<^sub>n = (\<lambda>M vm (to_remove, h). do {
+definition evsids_flush_int :: \<open>nat multiset \<Rightarrow> (nat,nat) ann_lits \<Rightarrow> (nat, double\<^sub>p) evsids \<Rightarrow> _ \<Rightarrow> ((nat, double\<^sub>p) evsids \<times> _)nres\<close> where
+\<open>evsids_flush_int \<A>\<^sub>i\<^sub>n = (\<lambda>M vm (to_remove, h). do {
     ASSERT(length to_remove \<le> unat32_max);
     (_, vm, h) \<leftarrow> WHILE\<^sub>T\<^bsup>\<lambda>(i, vm', h). i \<le> length to_remove \<and>
-          (i < length to_remove \<longrightarrow> vsids_push_literal_pre \<A>\<^sub>i\<^sub>n (to_remove!i) (vm'))\<^esup>
+          (i < length to_remove \<longrightarrow> evsids_push_literal_pre \<A>\<^sub>i\<^sub>n (to_remove!i) (vm'))\<^esup>
       (\<lambda>(i, vm, h). i < length to_remove)
       (\<lambda>(i, vm, h). do {
          ASSERT(i < length to_remove);
          ASSERT(to_remove!i \<in># \<A>\<^sub>i\<^sub>n);
          ASSERT(atoms_hash_del_pre (to_remove!i) h);
-         vm \<leftarrow> vsids_push_literal (to_remove!i) vm;
+         vm \<leftarrow> evsids_push_literal (to_remove!i) vm;
          RETURN (i+1, vm, atoms_hash_del (to_remove!i) h)})
       (0, vm, h);
     RETURN (vm, (emptied_list to_remove, h))
   })\<close>
 
 
-definition vsids_flush
-   :: \<open>nat multiset \<Rightarrow> (nat,nat) ann_lits \<Rightarrow> (nat, double\<^sub>p) vsids \<Rightarrow> nat set \<Rightarrow> ((nat, double\<^sub>p) vsids \<times> nat set) nres\<close>
+definition evsids_flush
+   :: \<open>nat multiset \<Rightarrow> (nat,nat) ann_lits \<Rightarrow> (nat, double\<^sub>p) evsids \<Rightarrow> nat set \<Rightarrow> ((nat, double\<^sub>p) evsids \<times> nat set) nres\<close>
 where
-  \<open>vsids_flush \<A>\<^sub>i\<^sub>n = (\<lambda>M vm remove_int. SPEC (\<lambda>x. (fst x) \<in> vsids \<A>\<^sub>i\<^sub>n M \<and> snd x = {}))\<close>
+  \<open>evsids_flush \<A>\<^sub>i\<^sub>n = (\<lambda>M vm remove_int. SPEC (\<lambda>x. (fst x) \<in> evsids \<A>\<^sub>i\<^sub>n M \<and> snd x = {}))\<close>
 
-lemma vsids_change_to_remove_order:
+lemma evsids_change_to_remove_order:
   assumes
-    vmtf: \<open>vc \<in> vsids \<A>\<^sub>i\<^sub>n M\<close> and
+    vmtf: \<open>vc \<in> evsids \<A>\<^sub>i\<^sub>n M\<close> and
     CD_rem: \<open>((C, D), to_remove) \<in> distinct_atoms_rel \<A>\<^sub>i\<^sub>n\<close> and
     nempty: \<open>isasat_input_nempty \<A>\<^sub>i\<^sub>n\<close> and
     bounded: \<open>isasat_input_bounded \<A>\<^sub>i\<^sub>n\<close> and
     t: \<open>to_remove \<subseteq> set_mset \<A>\<^sub>i\<^sub>n\<close>
-  shows \<open>vsids_flush_int \<A>\<^sub>i\<^sub>n M vc (C, D) \<le> \<Down>(Id \<times>\<^sub>r distinct_atoms_rel \<A>\<^sub>i\<^sub>n) (vsids_flush \<A>\<^sub>i\<^sub>n M vc to_remove)\<close>
+  shows \<open>evsids_flush_int \<A>\<^sub>i\<^sub>n M vc (C, D) \<le> \<Down>(Id \<times>\<^sub>r distinct_atoms_rel \<A>\<^sub>i\<^sub>n) (evsids_flush \<A>\<^sub>i\<^sub>n M vc to_remove)\<close>
 proof -
   have to_C: \<open>to_remove = set C\<close>
     using CD_rem by (auto simp: distinct_atoms_rel_def distinct_hash_atoms_rel_def)
@@ -254,39 +284,39 @@ proof -
       using simple_clss_size_upper_div2[OF bounded lits dist tauto]
       by (auto simp: unat32_max_def)
   qed
-  have acids_push_literal_pre: \<open>vsids_push_literal_pre \<A>\<^sub>i\<^sub>n (C ! i) vc\<close>
+  have acids_push_literal_pre: \<open>evsids_push_literal_pre \<A>\<^sub>i\<^sub>n (C ! i) vc\<close>
     if \<open>i < length C\<close> for i
-    using t that CD_rem unfolding vsids_push_literal_pre_def distinct_atoms_rel_def
+    using t that CD_rem unfolding evsids_push_literal_pre_def distinct_atoms_rel_def
       distinct_hash_atoms_rel_def by auto
-  define I where \<open>I \<equiv> \<lambda>(i::nat, vm'::(nat, double\<^sub>p)vsids, h). vm' \<in> vsids \<A>\<^sub>i\<^sub>n M \<and>
+  define I where \<open>I \<equiv> \<lambda>(i::nat, vm'::(nat, double\<^sub>p)evsids, h). vm' \<in> evsids \<A>\<^sub>i\<^sub>n M \<and>
     ((drop i C, h), to_remove - set (take i C)) \<in> distinct_atoms_rel \<A>\<^sub>i\<^sub>n \<and> i \<le> length C\<close>
 
   have sin: \<open>fst s < length (fst (C, D)) \<Longrightarrow> fst (C, D) ! fst s \<in># \<A>\<^sub>i\<^sub>n\<close> and
     atms: \<open>I s \<Longrightarrow> fst s < length (fst (C, D)) \<Longrightarrow> atoms_hash_del_pre (fst (C, D) ! fst s) (snd (snd s))\<close> for s
     using t CD_rem nth_mem[of \<open>fst s\<close> C]
-    unfolding vsids_push_literal_pre_def distinct_atoms_rel_def
+    unfolding evsids_push_literal_pre_def distinct_atoms_rel_def
       distinct_hash_atoms_rel_def I_def atoms_hash_del_pre_def atoms_hash_rel_def by (auto simp del: nth_mem)
 
   let ?R = \<open>measure (\<lambda>(i, vm', h). length C - i)\<close>
 
   have I_inv1_acids_push_literal_pre: \<open>I s \<Longrightarrow>
     fst (C, D) ! fst s \<in># \<A>\<^sub>i\<^sub>n \<Longrightarrow>
-    x \<in> vsids \<A>\<^sub>i\<^sub>n M \<Longrightarrow>
+    x \<in> evsids \<A>\<^sub>i\<^sub>n M \<Longrightarrow>
     fst (fst s + 1, x,
     atoms_hash_del (fst (C, D) ! fst s) (snd (snd s)))
     < length (fst (C, D)) \<Longrightarrow>
-    vsids_push_literal_pre \<A>\<^sub>i\<^sub>n
+    evsids_push_literal_pre \<A>\<^sub>i\<^sub>n
     (fst (C, D) ! fst (fst s + 1, x,
     atoms_hash_del (fst (C, D) ! fst s) (snd (snd s))))
     (fst (snd (fst s + 1, x, atoms_hash_del (fst (C, D) ! fst s) (snd (snd s)))))\<close>
     for s x
-    using t CD_rem unfolding vsids_push_literal_pre_def distinct_atoms_rel_def
+    using t CD_rem unfolding evsids_push_literal_pre_def distinct_atoms_rel_def
       distinct_hash_atoms_rel_def by auto
   have I_Suc: \<open>I s \<Longrightarrow>
     fst s < length (fst (C, D)) \<Longrightarrow>
     fst (C, D) ! fst s \<in># \<A>\<^sub>i\<^sub>n \<Longrightarrow>
     atoms_hash_del_pre (fst (C, D) ! fst s) (snd (snd s)) \<Longrightarrow>
-    x \<in> vsids \<A>\<^sub>i\<^sub>n M \<Longrightarrow>
+    x \<in> evsids \<A>\<^sub>i\<^sub>n M \<Longrightarrow>
     I (fst s + 1, x, atoms_hash_del (fst (C, D) ! fst s) (snd (snd s)))\<close>
     for s x
     apply (auto simp: I_def distinct_atoms_rel_def 
@@ -300,9 +330,9 @@ proof -
     done
 
   show ?thesis
-    unfolding vsids_flush_int_def vsids_flush_def case_prod_beta
+    unfolding evsids_flush_int_def evsids_flush_def case_prod_beta
     apply (refine_vcg specify_left[OF WHILEIT_rule_stronger_inv[where \<Phi> = \<open>(\<lambda>x. I x \<and> fst x =length (fst (C, D)))\<close> and I' = \<open>I\<close> and R = ?R]]
-      vsids_push_literal[where \<A>=\<A>\<^sub>i\<^sub>n and M=M])
+      evsids_push_literal[where \<A>=\<A>\<^sub>i\<^sub>n and M=M])
     subgoal by (rule length_le)
     subgoal by auto
     subgoal by auto
